## (1)

1. $0<x<1$时，$f_X(x)=\int_{-\infty}^{+\infty}f(x,y)\,\mathrm{d}y=\int_0^{2x}\,\mathrm{d}y=2x$
2. $x\leqslant0$或$x\geqslant1$,$f_X(x)=0$
3. $0<y<2$,$f_Y(y)=\int_{\frac{y}{2}}^1\,\mathrm{d}x=1-\frac{y}{2}$
4. $y\leqslant0$或$y\geqslant2$时，$f_Y(y)=0$

所以

$$
f_X(x)=\begin{cases}2x,0<x<1\\0,else\end{cases},f_Y(y)=\begin{cases}1-\frac{y}{2},0<y<2\\0,else\end{cases}
$$

## (2)

$$
F_Z(z)=P(Z\leqslant z)=P(2X-Y\leqslant z)=\iint_{2x-y\leqslant z}f(x,y)\,\mathrm{d}x\mathrm{d}y
$$

1. $z\leqslant0$或$z\geqslant2$时，$F_Z(z)=0\Longrightarrow f_Z(z)=0$
2. $0<z<2$时，$F_Z(z)=\int_0^{\frac{x}{2}}\,\mathrm{d}x\int_0^{2x}\,\mathrm{d}y+\int_{\frac{x}{2}}^1\,\mathrm{d}x\int_{2x-z}^{2x}\,\mathrm{d}y=z-\frac{z^2}{4}\Longrightarrow f_Z(z)=1-\frac{z}{2}$

于是

$$
f_Z(z)=\begin{cases}1-\frac{z}{2},0<z<2\\0,else\end{cases}
$$

## (3)

根据条件概率知

$$
P\left(Y\leqslant\frac{1}{2}\mid X\leqslant\frac{1}{2}\right)=\frac{P\left(Y\leqslant\frac{1}{2},X\leqslant\frac{1}{2}\right)}{P\left(X\leqslant\frac{1}{2}\right)}=\frac{\int_0^{\frac{1}{2}}\,\mathrm{d}y\int_{\frac{y}{2}}^{\frac{1}{2}}\,\mathrm{d}x}{\int_0^{\frac{1}{2}}2x\,\mathrm{d}x}=\frac{3}{4}
$$
