## (1)

因为$P\left(X^2=Y^2\right)=1$所以$P\left(X^2\neq Y^2\right)=0\Longrightarrow P\left(X=0,Y=1\right)+P\left(X=0,Y=-1\right)+P\left(X=1,Y=0\right)=0$,那么

$$
P\left(X=0,Y=1\right)=P\left(X=0,Y=-1\right)=P\left(X=1,Y=0\right)=0
$$

因为

$$
P\left(X=0\right)=P\left(X=0,Y=1\right)+P\left(X=0,Y=-1\right)+P\left(X=0,Y=0\right)
$$

所以

$$
P\left(X=0,Y=0\right)=\frac{1}{3},P\left(Y=1\right)=P\left(X=0,Y=1\right)+P\left(X=1,Y=1\right)
$$

因此

$$
P\left(X=1,Y=1\right)=\frac{1}{3},P\left(Y=-1\right)=P\left(X=0,Y=-1\right)+P\left(X=1,Y=-1\right)
$$

得到

$$
P\left(X=1,Y=-1\right)=\frac{1}{3}
$$

于是

所以有(行 Y 列 X)

|       |     $-1$      |      $0$      |      $1$      |     $P_i$     |
| :---: | :-----------: | :-----------: | :-----------: | :-----------: |
|  $0$  |      $0$      | $\frac{1}{3}$ |      $0$      | $\frac{1}{3}$ |
|  $1$  | $\frac{1}{3}$ |      $0$      | $\frac{1}{3}$ | $\frac{1}{3}$ |
| $P_j$ | $\frac{1}{3}$ | $\frac{1}{3}$ | $\frac{1}{3}$ |               |

## (2)

$Z=XY=-1,0,1$

$$
P\left(Z=-1\right)=P\left(X=1,Y=-1\right)=\frac{1}{3},P\left(Z=1\right)=P\left(X=1,Y=1\right)=\frac{1}{3}
$$

于是

$$
P\left(Z=0\right)=\frac{1}{3}
$$
