若$-1<x<1$

$$
f_X\left(x\right)=\int_{-\infty}^{+\infty}f\left(x,y\right)=\int_{x^2}^1\frac{21}{4}x^2\left(1-x^2\right)
$$

若$x\leqslant-1$或$x\geqslant1$，

$$
f_X\left(x\right)=0
$$

所以

$$
f_{Y\mid X}\left(y\mid x\right)=\frac{f\left(x,y\right)}{f_X\left(x\right)}=\begin{cases}\frac{2y}{1-x^4},-1<x<1,x^2\leqslant y\leqslant1\\0,其他\end{cases}
$$

于是

$$
P\left(Y\geqslant\frac{3}{4}\mid X=\frac{1}{2}\right)=1-P\left(Y<\frac{3}{4}\mid X=\frac{1}{2}\right)=1-\lim_{y\to\left(\frac{3}{4}\right)^-}\int_0^y\frac{2y}{1-\left(\frac{1}{2}\right)^4}\,\mathrm{d}y=\frac{2}{5}
$$
