$$
F_X\left(x\right)=F(x,+\infty)=\begin{cases}\lim\limits_{y\to+\infty}1-\mathrm{e}^{-\alpha x}=1-\mathrm{e}^{-\alpha x},x\geqslant0\\0,else\end{cases}
$$

$$
F_Y\left(y\right)=F\left(+\infty,y\right)=\begin{cases}\lim\limits_{x\to+\infty}\left(1-\mathrm{e}^{-\alpha x}\right)y=y,0\leqslant y\leqslant1\\\lim\limits_{x\to+\infty}1-\mathrm{e}^{-\alpha x}=1,y>1\\0,else\end{cases}
$$

1. $x\geqslant 0,0\leqslant y\leqslant1$时，$F_X(x)F_Y(y)=\left(1-\mathrm{e}^{-\alpha x}\right)y=F(x,y)$
2. $x\geqslant0,y>1$时，$F_X(x)F_Y(y)=1-\mathrm{e}^{-\alpha x}=F(x,y)$
3. else，$F_X(x)F_Y(y)=0=F(x,y)$
   因此$X$与$Y$相互独立
