## (1)

因为$Z$服从正态分布，且

$$
E(Z)=0,D(Z)=3\sigma^2\Longrightarrow Z\sim N\left(0,\left(\sqrt{3}\sigma\right)^2\right)
$$

于是概率密度

$$
f\left(z;\sigma^2\right)=\frac{1}{\sqrt{6\pi\sigma}}\mathrm{e}^{-\frac{z^2}{6\sigma^2}},-\infty<z< +\infty
$$

## (2)

似然函数

$$
L(\sigma^2)=\frac{1}{\left(\sqrt{6\pi}\right)^n\sigma^n}\mathrm{e}^{-\frac{\sum\limits_{i=1}^nz_i^2}{6\sigma^2}},-\infty<z<+\infty\Longrightarrow\ln{L\left(\sigma^2\right)}=-\frac{n}{2}\ln{6}\pi-n\ln{\sigma}-\frac{1}{6\sigma^2}\sum_{i=1}^nz_i^2
$$

令

$$
\frac{\mathrm{d}\ln{L\left(\sigma^2\right)}}{\mathrm{d}\left(\sigma^2\right)}=-\frac{n}{2\sigma^2}+\frac{1}{6\sigma^4}\sum_{i=1}^nz_i^2=0
$$

得

$$
\sigma^2=\frac{1}{3n}\sum_{i=1}^nz_i^2
$$

于是$\sigma^2$的最大似然估计量为

$$
\hat{\sigma}^2=\frac{1}{3n}\sum_{i=1}^nZ_i^2
$$

## (3)

因为

$$
E\left(\hat{\sigma}^2\right)=\frac{1}{3n}E\left(\sum_{i=1}^nZ_i^2\right)=\frac{1}{3}\left[D(Z)+\left(E(Z)\right)^2\right]=\sigma^2
$$

于是
$\hat{\sigma}^2$为$\sigma^2$的无偏估计量
